

# Backpropagation with Sigmoid and Binary Cross-Entropy (No Biases)

## 1. Forward definitions (no biases)

For layer  $\ell$  and unit  $j$  with inputs  $a_i^{\ell-1}$ :

$$z_j^\ell = \sum_i W_{ji}^\ell a_i^{\ell-1}, \quad a_j^\ell = \sigma(z_j^\ell), \quad \sigma(u) = \frac{1}{1 + e^{-u}}, \quad \sigma'(u) = \sigma(u)(1 - \sigma(u)).$$

## 2. Loss at the output (binary cross-entropy)

For the output layer  $L$  with independent sigmoid outputs  $a_j^L$  and targets  $t_j$ :

$$\mathcal{L} = - \sum_j \left( t_j \log a_j^L + (1 - t_j) \log(1 - a_j^L) \right).$$

## 3. Gradient at the output layer

We seek the derivative w.r.t. the *pre-activation*  $z_j^L$ :

$$\delta_j^L \equiv \frac{\partial \mathcal{L}}{\partial z_j^L}.$$

Apply the chain rule:

$$\frac{\partial \mathcal{L}}{\partial z_j^L} = \frac{\partial \mathcal{L}}{\partial a_j^L} \cdot \frac{\partial a_j^L}{\partial z_j^L}.$$

Each factor is

$$\frac{\partial \mathcal{L}}{\partial a_j^L} = -\frac{t_j}{a_j^L} + \frac{1 - t_j}{1 - a_j^L}, \quad \frac{\partial a_j^L}{\partial z_j^L} = \sigma'(z_j^L) = a_j^L(1 - a_j^L).$$

Multiplying and simplifying gives the familiar result

$$\boxed{\delta_j^L = a_j^L - t_j}$$

(i.e., the sigmoid derivative cancels with the BCE term via the chain rule).

## 4. Propagating to a hidden layer via the chain rule

Start from the forward relation of the next layer:

$$z_k^{\ell+1} = \sum_j W_{kj}^{\ell+1} a_j^\ell.$$

For a hidden unit  $j$  in layer  $\ell$ ,

$$\frac{\partial \mathcal{L}}{\partial z_j^\ell} = \sum_k \underbrace{\frac{\partial \mathcal{L}}{\partial z_k^{\ell+1}}}_{\delta_k^{\ell+1}} \underbrace{\frac{\partial z_k^{\ell+1}}{\partial a_j^\ell}}_{W_{kj}^{\ell+1}} \underbrace{\frac{\partial a_j^\ell}{\partial z_j^\ell}}_{\sigma'(z_j^\ell)} = \sum_k \delta_k^{\ell+1} W_{kj}^{\ell+1} \sigma'(z_j^\ell).$$

Using  $\sigma'(z_j^\ell) = a_j^\ell(1 - a_j^\ell)$ , the hidden-layer delta becomes

$$\delta_j^\ell = \left( \sum_k W_{kj}^{\ell+1} \delta_k^{\ell+1} \right) a_j^\ell(1 - a_j^\ell).$$

## 5. Gradients w.r.t. the weights (no biases)

From  $z_j^\ell = \sum_i W_{ji}^\ell a_i^{\ell-1}$ ,

$$\frac{\partial \mathcal{L}}{\partial W_{ji}^\ell} = \frac{\partial \mathcal{L}}{\partial z_j^\ell} \cdot \frac{\partial z_j^\ell}{\partial W_{ji}^\ell} = \delta_j^\ell a_i^{\ell-1}.$$

A plain gradient-descent update with learning rate  $\eta$  is

$$W_{ji}^\ell \leftarrow W_{ji}^\ell - \eta \frac{\partial \mathcal{L}}{\partial W_{ji}^\ell} = W_{ji}^\ell - \eta \delta_j^\ell a_i^{\ell-1}.$$

## 6. Minimal backprop recipe (index form)

1. Forward: compute all  $z_j^\ell$  and  $a_j^\ell$  for  $\ell = 1, \dots, L$ .
2. Output deltas:  $\delta_j^L = a_j^L - t_j$ .
3. For  $\ell = L - 1$  down to 1:  $\delta_j^\ell = \left( \sum_k W_{kj}^{\ell+1} \delta_k^{\ell+1} \right) a_j^\ell(1 - a_j^\ell)$ .
4. Gradients:  $\frac{\partial \mathcal{L}}{\partial W_{ji}^\ell} = \delta_j^\ell a_i^{\ell-1}$ .